Outline Proof Correctness Message Body
Includes all requirements, expected function definitions. Avoids arithmetic problems in EncryptMessageBody method

src/SDK/MessageBody.dfy
@@ -13,7 +13,9 @@ module MessageBody {
     provides EncryptMessageBody
     provides DecryptFramedMessageBody, DecryptNonFramedMessageBody
     provides StandardLibrary, UInt, Msg, AlgorithmSuite, Materials, Streams
-
+    provides FramesToSequence, FrameToSubsequence
+    reveals Frame
+    
   import opened StandardLibrary
   import opened UInt = StandardLibrary.UInt
   import AlgorithmSuite
@@ -25,6 +27,8 @@ module MessageBody {
   import UTF8
 
   datatype BodyAADContent = RegularFrame | FinalFrame | SingleBlock
+  datatype Frame = RegFrameCons(seqNumb: uint32, iv: seq<uint8>, encCont: seq<uint8>, authTag: seq<uint8>) |
+                   FinalFrameCons(seqNumbEnd: uint32, seqNumb: uint32, iv: seq<uint8>, encContLength: uint32, encCont: seq<uint8>, authTag: seq<uint8>)
 
   const BODY_AAD_CONTENT_REGULAR_FRAME: string := "AWSKMSEncryptionClient Frame"
   const BODY_AAD_CONTENT_FINAL_FRAME: string := "AWSKMSEncryptionClient Final Frame"
@@ -41,14 +45,101 @@ module MessageBody {
   const ENDFRAME_SEQUENCE_NUMBER: uint32 := 0xFFFF_FFFF
   const NONFRAMED_SEQUENCE_NUMBER: uint32 := 1
 
+  //Parses a sequence encoding a regular frame to a regular frame datastructure
+  function SubsequenceToRegFrame(xs: seq<uint8>, algorithmSuiteID: AlgorithmSuite.ID,frameLength: int): (f: Frame)
+    requires |xs| == 4 + algorithmSuiteID.IVLength() + frameLength + algorithmSuiteID.TagLength();
+    requires 0 < frameLength < UINT32_LIMIT
+    requires 0 <= algorithmSuiteID.IVLength()
+    ensures f.RegFrameCons?
+    ensures |f.iv| == algorithmSuiteID.IVLength()
+    ensures |f.encCont| == frameLength;
+    ensures |f.authTag| == algorithmSuiteID.TagLength()
+    ensures FrameToSubsequence(f) == xs
+  {
+    var sqn := SeqToUInt32(xs[0..4]);
+    var ivEnd := algorithmSuiteID.IVLength() +  4;
+    var encryptEnd := ivEnd + frameLength;
+    RegFrameCons(sqn,xs[4..ivEnd],xs[ivEnd..ivEnd+encryptEnd],xs[encryptEnd..])
+  }
+
+  //Parses a sequence encoding a final frame to a final frame datastructure
+  function SubsequenceToFinalFrame(xs: seq<uint8>, algorithmSuiteID: AlgorithmSuite.ID, frameLength: int): (f: Frame)
+    requires 4 + 4 + algorithmSuiteID.IVLength() + 4 + algorithmSuiteID.TagLength() <= |xs| <= 4 + 4 + algorithmSuiteID.IVLength() + 4 + frameLength + algorithmSuiteID.TagLength();
+    requires 0 <= algorithmSuiteID.IVLength();
+    requires 0 < frameLength < UINT32_LIMIT
+    requires var fl : uint32 := SeqToUInt32(xs[4+4+algorithmSuiteID.IVLength()..4+4+algorithmSuiteID.IVLength()+4]);
+             0 <= fl <= frameLength as uint32 &&
+             |xs| == 4 + 4 + algorithmSuiteID.IVLength() + 4 + fl as int + algorithmSuiteID.TagLength() 
+    requires 0 < algorithmSuiteID.TagLength()
+    ensures f.FinalFrameCons?
+    ensures |f.iv| == algorithmSuiteID.IVLength()
+    ensures |f.iv| == algorithmSuiteID.IVLength()
+    ensures |f.encCont| == frameLength;
+    ensures |f.authTag| == algorithmSuiteID.TagLength()
+    ensures FrameToSubsequence(f) == xs
+  {
+    var sqnE := SeqToUInt32(xs[0..4]);
+    var sqn := SeqToUInt32(xs[4..8]);
+    var ivEnd := algorithmSuiteID.IVLength() as uint32 +  8;
+    var fl := SeqToUInt32(xs[ivEnd..ivEnd+4]);
+    var encryptEnd := 4 + 4 + algorithmSuiteID.IVLength() + 4 + fl as int + algorithmSuiteID.TagLength() as int;
+    FinalFrameCons(sqnE,sqn,xs[8..ivEnd],fl,xs[ivEnd+4..encryptEnd],xs[encryptEnd..])
+  }
+
+  //Converts sequence of Frames to a sequence encoding all frames
+  function FramesToSequence(fs : seq<Frame>): (xs: seq<uint8>)
+    requires |fs| <= UINT32_LIMIT
+  {
+    if fs == [] then
+      []
+    else
+      FrameToSubsequence(fs[0]) + FramesToSequence(fs[1..])
+  }
+
+  //Converts Frame to a sequence encoding a frame
+  function FrameToSubsequence(f : Frame): (xs: seq<uint8>)
+    ensures |xs| <= UINT32_LIMIT
+  {
+    match f 
+      case RegFrameCons(seqNumb, iv, encCont, authTag) =>
+        var seqNumSeq := UInt32ToSeq(seqNumb);
+        seqNumSeq + iv + encCont + authTag
+
+      case FinalFrameCons(seqNumbEnd, seqNumb, iv, encContLength, encCont, authTag) =>
+        var seqNumbEndSeq := UInt32ToSeq(seqNumbEnd);
+        var seqNumbSeq := UInt32ToSeq(seqNumb);
+        var encContLengthSeq := seq(4 - |UInt32ToSeq(encContLength)|, _ => 0) + UInt32ToSeq(encContLength);
+        seqNumbEndSeq + seqNumbSeq + iv + encContLengthSeq + encContLengthSeq + authTag
+  }
+
+
   method EncryptMessageBody(plaintext: seq<uint8>, frameLength: int, messageID: Msg.MessageID, key: seq<uint8>, algorithmSuiteID: AlgorithmSuite.ID) returns (res: Result<seq<uint8>>)
     requires |key| == algorithmSuiteID.KeyLength()
     requires 0 < frameLength < UINT32_LIMIT
-  {
+    requires frameLength > 0
+    ensures match res
+      case Failure(e) => true
+      case Success(resS) => exists fs: seq<Frame> :: 
+           0 < |fs| < UINT32_LIMIT    
+        && FramesToSequence(fs) == resS
+        && fs[|fs| - 1].FinalFrameCons?
+        && 0 <= fs[|fs|-1].encContLength as int <= frameLength 
+        && forall f | f in fs[..|fs| - 1] :: f.RegFrameCons?
+        && forall f | f in fs[..|fs| - 1] :: frameLength == |f.encCont|
+        && fs[0].seqNumb == 1
+        && fs[|fs|-1].seqNumbEnd as int == |fs|
+        && forall i | 0 <= i < |fs| - 1 :: fs[i+1].seqNumb as int == fs[i].seqNumb as int + 1
+        && forall f1,f2 | f1 in fs && f2 in fs && f1 != f2 :: f1.iv != f2.iv
+        && |plaintext| < frameLength ==> |fs| == 1 && fs[0].FinalFrameCons?  
+  { 
     var body := [];
-    var n, sequenceNumber := 0, START_SEQUENCE_NUMBER;
+    var n : int, sequenceNumber := 0, START_SEQUENCE_NUMBER;
+    
+    ghost var fres : seq<Frame> := [];
+    
     while n + frameLength < |plaintext|
-      invariant 0 <= n <= |plaintext|
+      invariant |plaintext| != 0 ==> 0 <= n < |plaintext|
+      invariant |plaintext| == 0 ==> 0 == n
       invariant START_SEQUENCE_NUMBER <= sequenceNumber <= ENDFRAME_SEQUENCE_NUMBER
     {
       if sequenceNumber == ENDFRAME_SEQUENCE_NUMBER {
@@ -56,11 +147,17 @@ module MessageBody {
       }
       var plaintextFrame := plaintext[n..n + frameLength];
       var regularFrame :- EncryptRegularFrame(algorithmSuiteID, key, frameLength, messageID, plaintextFrame, sequenceNumber);
+      
+      fres := fres + [SubsequenceToRegFrame(regularFrame, algorithmSuiteID, frameLength)];
       body := body + regularFrame;
       n, sequenceNumber := n + frameLength, sequenceNumber + 1;
     }
+
     var finalFrame :- EncryptFinalFrame(algorithmSuiteID, key, frameLength, messageID, plaintext[n..], sequenceNumber);
     body := body + finalFrame;
+    
+    fres := fres + [SubsequenceToFinalFrame(finalFrame, algorithmSuiteID, frameLength)];
+    
     return Success(body);
   }
 
@@ -72,6 +169,15 @@ module MessageBody {
     requires |plaintext| < UINT32_LIMIT
     requires |plaintext| == frameLength && sequenceNumber != ENDFRAME_SEQUENCE_NUMBER
     requires 4 <= algorithmSuiteID.IVLength()
+    ensures match res 
+      case Failure(e) => true
+      case Success(resS) => 
+        |resS| == 4 + algorithmSuiteID.IVLength() + frameLength + algorithmSuiteID.TagLength() &&
+        var iv := seq(algorithmSuiteID.IVLength() - 4, _ => 0) + UInt32ToSeq(sequenceNumber);
+        var encCont := resS[4 + algorithmSuiteID.IVLength() ..4 + algorithmSuiteID.IVLength() + frameLength]; //Is there a better way to do this
+        var authTag := resS[4 + algorithmSuiteID.IVLength() + frameLength..];
+        var frame := RegFrameCons(sequenceNumber, iv, encCont, authTag);
+        FrameToSubsequence(frame) == resS
   {
     var seqNumSeq := UInt32ToSeq(sequenceNumber);
     var unauthenticatedFrame := seqNumSeq;
@@ -96,22 +202,31 @@ module MessageBody {
     requires |plaintext| < UINT32_LIMIT
     requires |plaintext| <= frameLength
     requires 4 <= algorithmSuiteID.IVLength()
+    ensures match res 
+      case Failure(e) => true
+      case Success(resS) => 
+            |resS| == 4 + 4 + algorithmSuiteID.IVLength() + 4 + |plaintext| + algorithmSuiteID.TagLength()
+        &&  |plaintext| == SeqToUInt32(resS[4 + 4 + algorithmSuiteID.IVLength()..4 + 4 + algorithmSuiteID.IVLength() + 4]) as int &&
+        var iv := seq(algorithmSuiteID.IVLength() - 4, _ => 0) + UInt32ToSeq(sequenceNumber);
+        var encCont := resS[4 + 4 + algorithmSuiteID.IVLength() + 4 .. 4 + 4 + algorithmSuiteID.IVLength() + 4 + |plaintext|]; //Is there a better way to do this
+        var authTag := resS[4 + 4 + algorithmSuiteID.IVLength() + 4 + |plaintext|..];
+        var frame := FinalFrameCons(ENDFRAME_SEQUENCE_NUMBER, sequenceNumber, iv, |plaintext| as uint32, encCont, authTag);
+            FrameToSubsequence(frame) == resS
   {
     var unauthenticatedFrame := UInt32ToSeq(ENDFRAME_SEQUENCE_NUMBER);
     var seqNumSeq := UInt32ToSeq(sequenceNumber);
     unauthenticatedFrame := unauthenticatedFrame + seqNumSeq;
-
+    
     var iv := seq(algorithmSuiteID.IVLength() - 4, _ => 0) + UInt32ToSeq(sequenceNumber);
     SeqWithUInt32Suffix(iv, sequenceNumber as nat);  // this proves SeqToNat(iv) == sequenceNumber as nat
     unauthenticatedFrame := unauthenticatedFrame + iv;
-
     unauthenticatedFrame := unauthenticatedFrame + UInt32ToSeq(|plaintext| as uint32);
-
+    
     var aad := BodyAAD(messageID, FinalFrame, sequenceNumber, |plaintext| as uint64);
-
+    
     var encryptionOutput :- AESEncryption.AESEncrypt(algorithmSuiteID.EncryptionSuite(), iv, key, plaintext, aad);
     unauthenticatedFrame := unauthenticatedFrame + encryptionOutput.cipherText + encryptionOutput.authTag;
-
+    
     return Success(unauthenticatedFrame);
   }
 
